Next proofs

compiler/backend/proofs/word_cseProofScript.sml
@@ -9,19 +9,31 @@ val _ = new_theory "word_cseProof";
 val _ = set_grammar_ancestry ["wordLang", "wordSem", "wordProps", "word_cse"];
 
 Definition data_inv_def:
-  data_inv (data:knowledge) (s:('a,'c,'ffi) wordSem$state) = T
+  data_inv (data:knowledge) (s:('a,'c,'ffi) wordSem$state) ⇔
+    (∀r v. lookup r data.inst_map = SOME v ⇒ get_var r s = get_var v s) ∧
+    (∀r v. lookup r data.och_map = SOME v ⇒ get_var r s = get_var v s)
 End
+
+Theorem canonicalRegs_correct[simp]:
+  ∀data r s. data_inv data s ⇒ get_var (canonicalRegs data r) s = get_var r s
+Proof
+  rpt strip_tac \\
+  gvs [data_inv_def, canonicalRegs_def] \\
+  fs [lookup_any_def] \\
+  Cases_on ‘lookup r data.inst_map’ \\ fs [] \\
+  Cases_on ‘lookup r data.och_map’ \\ fs []
+QED
 
 (* setting up the goal *)
 
 val goal = “
-   λ(p:'a wordLang$prog,s:('a,'c,'ffi) wordSem$state).
-     ∀res s' data p' data'.
-       evaluate (p, s) = (res, s') ∧ flat_exp_conventions p ∧
-       data_inv data s ∧
-       word_cse data p  = (data', p') ⇒
-         evaluate (p', s) = (res, s') ∧
-         (res = NONE ⇒ data_inv data' s')”
+ λ(p:'a wordLang$prog,s:('a,'c,'ffi) wordSem$state).
+   ∀res s' data p' data'.
+     evaluate (p, s) = (res, s') ∧ flat_exp_conventions p ∧
+     data_inv data s ∧
+     word_cse data p  = (data', p') ⇒
+     evaluate (p', s) = (res, s') ∧
+     (res = NONE ⇒ data_inv data' s')”
 
 local
   val gst = goal |> Ho_Rewrite.PURE_ONCE_REWRITE_CONV [Once PFORALL_THM] |> concl |> rhs
@@ -31,22 +43,23 @@ in
   fun get_goal s = first (can (find_term (can (match_term (Term [QUOTE s]))))) ind_goals
   fun compile_correct_tm () = ind_thm |> concl |> rand
   fun the_ind_thm () = ind_thm
-end
+end;
 
 (* proof of the cases *)
 
 Theorem comp_Skip_correct:
   ^(get_goal "Skip")
 Proof
-  rpt strip_tac \\
-  fs[word_cse_def]
+  gvs[word_cse_def, evaluate_def]
 QED
 
 Theorem comp_Alloc_correct:
   ^(get_goal "Alloc")
 Proof
-  rpt strip_tac \\
-  fs[word_cse_def]
+  gvs[word_cse_def, data_inv_def, lookup_def, evaluate_def] \\
+  gvs [AllCaseEqs()] \\
+  cheat
+  (* TODO make alloc forget everything for now *)
 QED
 
 Theorem comp_Move_correct:
@@ -74,15 +87,16 @@ QED
 Theorem comp_Get_correct:
   ^(get_goal "Get")
 Proof
-  rpt strip_tac \\
-  fs[word_cse_def]
+  gvs[word_cse_def, data_inv_def, evaluate_def] \\
+  gvs[AllCaseEqs(), PULL_EXISTS] \\
+  cheat
 QED
 
 Theorem comp_Set_correct:
   ^(get_goal "wordLang$Set")
 Proof
-  rpt strip_tac \\
-  fs[word_cse_def]
+  cheat
+  (*gvs[word_cse_def, data_inv_def]*)
 QED
 
 Theorem comp_OpCurrHeap_correct:
@@ -100,21 +114,29 @@ QED
 Theorem comp_Tick_correct:
   ^(get_goal "Tick")
 Proof
-  rpt strip_tac \\
-  fs[word_cse_def]
+  gvs[word_cse_def, data_inv_def, evaluate_def] \\
+  rw [] \\
+  fs [get_var_def, dec_clock_def]
 QED
 
 Theorem comp_MustTerminate_correct:
   ^(get_goal "MustTerminate")
 Proof
-  rpt strip_tac \\
+  rpt gen_tac \\
+  strip_tac \\
+  rpt gen_tac \\
   gs[word_cse_def] \\
   pairarg_tac \\ gvs [evaluate_def,flat_exp_conventions_def] \\
   gvs [AllCaseEqs()] \\
+  strip_tac
+  >- gvs [evaluate_def] \\
   pairarg_tac \\ gvs [] \\
-  pairarg_tac \\ gvs [] \\
-  first_x_assum drule \\
-  gvs []
+  first_x_assum (drule_at Any) \\
+  impl_tac
+  >- fs [data_inv_def, get_var_def] \\
+  fs [evaluate_def] \\
+  rw [] \\
+  gvs [AllCaseEqs(), data_inv_def, get_var_def]
 QED
 
 Theorem comp_Seq_correct:
@@ -139,54 +161,69 @@ QED
 Theorem comp_Return_correct:
   ^(get_goal "Return")
 Proof
-  fs[word_cse_def]
+  fs[word_cse_def, evaluate_def, flat_exp_conventions_def]
+  \\ rw []
+  \\ gvs [AllCaseEqs()]
 QED
 
 Theorem comp_Raise_correct:
   ^(get_goal "wordLang$Raise")
 Proof
-  fs[word_cse_def]
+  fs[word_cse_def, evaluate_def, flat_exp_conventions_def]
+  \\ rw []
+  \\ gvs [AllCaseEqs()]
+
 QED
 
 Theorem comp_If_correct:
   ^(get_goal "wordLang$If")
 Proof
-  cheat
+  rpt gen_tac
+  \\ strip_tac
+  \\ rpt gen_tac
+  \\ simp_tac std_ss [evaluate_def, AllCaseEqs(), word_cse_def, LET_THM]
+  \\ rpt (pairarg_tac \\ simp [])
+  \\ strip_tac
+  \\ gvs [evaluate_def]
+  \\ ‘get_var_imm (canonicalImmReg data ri) s = get_var_imm ri s’ by
+    (Cases_on ‘ri’ \\ fs [get_var_imm_def, canonicalImmReg_def])
+  \\ fs [flat_exp_conventions_def]
+  \\ first_x_assum drule_all
+  \\ rw []
+  \\ simp [data_inv_def, empty_data_def, get_var_def, lookup_def]
 QED
 
 Theorem comp_LocValue_correct:
   ^(get_goal "wordLang$LocValue")
 Proof
-  rpt strip_tac \\
-  fs[word_cse_def]
+  gvs[word_cse_def, data_inv_def]
+  \\ cheat
 QED
+
+(* DATA EMPTY *)
 
 Theorem comp_Install_correct:
   ^(get_goal "wordLang$Install")
 Proof
-  rpt strip_tac \\
-  fs[word_cse_def]
+  gvs[word_cse_def, data_inv_def]
 QED
 
 Theorem comp_CodeBufferWrite_correct:
   ^(get_goal "wordLang$CodeBufferWrite")
 Proof
-  rpt strip_tac \\
-  fs[word_cse_def]
+  gvs[word_cse_def, data_inv_def]
 QED
 
 Theorem comp_DataBufferWrite_correct:
   ^(get_goal "wordLang$DataBufferWrite")
 Proof
-  rpt strip_tac \\
-  fs[word_cse_def]
+  gvs[word_cse_def, data_inv_def]
 QED
 
 Theorem comp_FFI_correct:
   ^(get_goal "wordLang$FFI")
 Proof
-  rpt strip_tac \\
-  fs[word_cse_def]
+  gvs[word_cse_def, data_inv_def, evaluate_def]
 QED
 
 Theorem comp_Call_correct:
@@ -194,6 +231,8 @@ Theorem comp_Call_correct:
 Proof
   fs[word_cse_def]
 QED
+
+(* DATA EMPTY *)
 
 Theorem comp_correct:
   ^(compile_correct_tm ())
